WIP, spec + compilation done and ladderstep proof started

src/Bedrock/Field/Interface/Compilation.v
@@ -9,9 +9,6 @@ Section Compile.
   Context {field_parameters : FieldParameters}
           {field_representaton : FieldRepresentation}
           {field_representation_ok : FieldRepresentation_ok}.
-  Existing Instances spec_of_mul spec_of_add spec_of_sub spec_of_square
-           spec_of_scmula24 spec_of_inv spec_of_felem_copy
-           spec_of_felem_small_literal.
 
   (* "Hidden" alias protects a Placeholder (e.g. the pointer reserved for the
      final output value) from having intermediate values stored in it *)
@@ -26,448 +23,184 @@ Section Compile.
     end; eauto;
     sepsimpl; repeat straightline'; subst; eauto.
 
-  Lemma compile_mul :
-    forall (locals: Semantics.locals) (mem: Semantics.mem)
-           (locals_ok : Semantics.locals -> Prop)
-      tr retvars R Rin Rout functions T (pred: T -> list word -> Semantics.mem -> Prop)
-      (x y : felem) x_ptr x_var y_ptr y_var out_ptr out_var
-      (X Y : F M_pos) k k_impl,
-      spec_of_mul functions ->
-      bounded_by loose_bounds x ->
-      bounded_by loose_bounds y ->
-      feval x = X ->
-      feval y = Y ->
-      (FElem x_ptr x * FElem y_ptr y * Rin)%sep mem ->
+  Lemma compile_binop {name} {op: BinOp name}
+        {tr mem locals functions} x y:
+    let v := bin_model (feval x) (feval y) in
+    forall {P} {pred: P v -> predicate} {k: nlet_eq_k P v} {k_impl}
+      Rin Rout x_ptr x_var y_ptr y_var out_ptr out_var,
+
+      (_: spec_of name) functions ->
+      bounded_by bin_xbounds x ->
+      bounded_by bin_ybounds y ->
+
+      map.get locals out_var = Some out_ptr ->
       (Placeholder out_ptr * Rout)%sep mem ->
+
+      (FElem x_ptr x * FElem y_ptr y * Rin)%sep mem ->
       map.get locals x_var = Some x_ptr ->
       map.get locals y_var = Some y_ptr ->
-      map.get locals out_var = Some out_ptr ->
-      let v := (X * Y)%F in
-      (let head := v in
-       forall out m,
-         feval out = head ->
-         bounded_by tight_bounds out ->
+
+      (let v := v in
+       forall out m (Heq: feval out = v),
+         bounded_by bin_outbounds out ->
          sep (FElem out_ptr out) Rout m ->
-         (find k_impl
-          implementing (pred (k head))
-          and-returning retvars
-          and-locals-post locals_ok
-          with-locals locals and-memory m and-trace tr and-rest R
-          and-functions functions)) ->
-      (let head := v in
-       find (cmd.seq
-               (cmd.call [] mul [expr.var out_var; expr.var x_var;
-                                   expr.var y_var])
-               k_impl)
-       implementing (pred (dlet head k))
-       and-returning retvars
-       and-locals-post locals_ok
-       with-locals locals and-memory mem and-trace tr and-rest R
-       and-functions functions).
+         (<{ Trace := tr;
+             Memory := m;
+             Locals := locals;
+             Functions := functions }>
+          k_impl
+          <{ pred (k v eq_refl) }>)) ->
+      <{ Trace := tr;
+         Memory := mem;
+         Locals := locals;
+         Functions := functions }>
+      cmd.seq
+        (cmd.call [] name [expr.var x_var; expr.var y_var;
+                          expr.var out_var])
+        k_impl
+      <{ pred (nlet_eq [out_var] v k) }>.
   Proof. prove_field_compilation. Qed.
 
-  Lemma compile_add :
-    forall (locals: Semantics.locals) (mem: Semantics.mem)
-           (locals_ok : Semantics.locals -> Prop)
-      tr retvars R Rin Rout functions T (pred: T -> list word -> Semantics.mem -> Prop)
-      (x y : felem) x_ptr x_var y_ptr y_var out_ptr out_var
-      (X Y : F M_pos) k k_impl,
-      spec_of_add functions ->
-      bounded_by tight_bounds x ->
-      bounded_by tight_bounds y ->
-      feval x = X ->
-      feval y = Y ->
-      (FElem x_ptr x * FElem y_ptr y * Rin)%sep mem ->
+  Lemma compile_unop {name} (op: UnOp name) {tr mem locals functions} x:
+    let v := un_model (feval x) in
+    forall {P} {pred: P v -> predicate} {k: nlet_eq_k P v} {k_impl}
+      Rin Rout x_ptr x_var out_ptr out_var,
+
+      (_: spec_of name) functions ->
+      bounded_by un_xbounds x ->
+
+      map.get locals out_var = Some out_ptr ->
       (Placeholder out_ptr * Rout)%sep mem ->
-      map.get locals x_var = Some x_ptr ->
-      map.get locals y_var = Some y_ptr ->
-      map.get locals out_var = Some out_ptr ->
-      let v := (X + Y)%F in
-      (let head := v in
-       forall out m,
-         feval out = head ->
-         bounded_by loose_bounds out ->
-         sep (FElem out_ptr out) Rout m ->
-         (find k_impl
-          implementing (pred (k head))
-          and-returning retvars
-          and-locals-post locals_ok
-          with-locals locals and-memory m and-trace tr and-rest R
-          and-functions functions)) ->
-      (let head := v in
-       find (cmd.seq
-               (cmd.call [] add [expr.var out_var; expr.var x_var;
-                                   expr.var y_var])
-               k_impl)
-       implementing (pred (dlet head k))
-       and-returning retvars
-       and-locals-post locals_ok
-       with-locals locals and-memory mem and-trace tr and-rest R
-       and-functions functions).
-  Proof. prove_field_compilation. Qed.
 
-  Lemma compile_sub :
-    forall (locals: Semantics.locals) (mem: Semantics.mem)
-           (locals_ok : Semantics.locals -> Prop)
-      tr retvars R Rin Rout functions T (pred: T -> list word -> Semantics.mem -> Prop)
-      (x y : felem) x_ptr x_var y_ptr y_var out_ptr out_var
-      (X Y : F M_pos) k k_impl,
-      spec_of_sub functions ->
-      bounded_by tight_bounds x ->
-      bounded_by tight_bounds y ->
-      feval x = X ->
-      feval y = Y ->
-      (FElem x_ptr x * FElem y_ptr y * Rin)%sep mem ->
-      (Placeholder out_ptr * Rout)%sep mem ->
-      map.get locals x_var = Some x_ptr ->
-      map.get locals y_var = Some y_ptr ->
-      map.get locals out_var = Some out_ptr ->
-      let v := (X - Y)%F in
-      (let head := v in
-       forall out m,
-         feval out = head ->
-         bounded_by loose_bounds out ->
-         sep (FElem out_ptr out) Rout m ->
-         (find k_impl
-          implementing (pred (k head))
-          and-returning retvars
-          and-locals-post locals_ok
-          with-locals locals and-memory m and-trace tr and-rest R
-          and-functions functions)) ->
-      (let head := v in
-       find (cmd.seq
-               (cmd.call [] sub [expr.var out_var; expr.var x_var;
-                                   expr.var y_var])
-               k_impl)
-       implementing (pred (dlet head k))
-       and-returning retvars
-       and-locals-post locals_ok
-       with-locals locals and-memory mem and-trace tr and-rest R
-       and-functions functions).
-  Proof. prove_field_compilation. Qed.
-
-  Lemma compile_square :
-    forall (locals: Semantics.locals) (mem: Semantics.mem)
-           (locals_ok : Semantics.locals -> Prop)
-      tr retvars R Rin Rout functions T (pred: T -> list word -> Semantics.mem -> Prop)
-      (x : felem) x_ptr x_var out_ptr out_var (X : F M_pos) k k_impl,
-      spec_of_square functions ->
-      bounded_by loose_bounds x ->
-      feval x = X ->
       (FElem x_ptr x * Rin)%sep mem ->
-      (Placeholder out_ptr * Rout)%sep mem ->
       map.get locals x_var = Some x_ptr ->
-      map.get locals out_var = Some out_ptr ->
-      let v := (X ^ 2)%F in
-      (let head := v in
-       forall out m,
-         feval out = head ->
-         bounded_by tight_bounds out ->
-         sep (FElem out_ptr out) Rout m ->
-         (find k_impl
-          implementing (pred (k head))
-          and-returning retvars
-          and-locals-post locals_ok
-          with-locals locals and-memory m and-trace tr and-rest R
-          and-functions functions)) ->
-      (let head := v in
-       find (cmd.seq
-               (cmd.call [] square [expr.var out_var; expr.var x_var])
-               k_impl)
-       implementing (pred (dlet head k))
-       and-returning retvars
-       and-locals-post locals_ok
-       with-locals locals and-memory mem and-trace tr and-rest R
-       and-functions functions).
-  Proof.
-    intros. subst_lets_in_goal.
-    rewrite F.pow_2_r in *.
-    prove_field_compilation.
-  Qed.
 
-  Lemma compile_scmula24 :
-    forall (locals: Semantics.locals) (mem: Semantics.mem)
-           (locals_ok : Semantics.locals -> Prop)
-      tr retvars R Rin Rout functions T (pred: T -> list word -> Semantics.mem -> Prop)
-      (x : felem) x_ptr x_var out_ptr out_var (X : F M_pos) k k_impl,
-      spec_of_scmula24 functions ->
-      bounded_by loose_bounds x ->
-      feval x = X ->
-      (FElem x_ptr x * Rin)%sep mem ->
-      (Placeholder out_ptr * Rout)%sep mem ->
-      map.get locals x_var = Some x_ptr ->
-      map.get locals out_var = Some out_ptr ->
-      let v := (a24 * X)%F in
-      (let head := v in
+      (let v := v in
        forall out m,
-         feval out = head ->
-         bounded_by tight_bounds out ->
+         bounded_by un_outbounds out ->
          sep (FElem out_ptr out) Rout m ->
-         (find k_impl
-          implementing (pred (k head))
-          and-returning retvars
-          and-locals-post locals_ok
-          with-locals locals and-memory m and-trace tr and-rest R
-          and-functions functions)) ->
-      (let head := v in
-       find (cmd.seq
-               (cmd.call [] scmula24 [expr.var out_var; expr.var x_var])
-               k_impl)
-       implementing (pred (dlet head k))
-       and-returning retvars
-       and-locals-post locals_ok
-       with-locals locals and-memory mem and-trace tr and-rest R
-       and-functions functions).
+         (<{ Trace := tr;
+             Memory := m;
+             Locals := locals;
+             Functions := functions }>
+          k_impl
+          (* <{ (rew [fun v => P v -> predicate)] Heq in pred) (k (eval out mod M) Heq) }>)) -> *)
+          <{ pred (k v eq_refl) }>)) ->
+      <{ Trace := tr;
+         Memory := mem;
+         Locals := locals;
+         Functions := functions }>
+      cmd.seq
+        (cmd.call [] name [expr.var x_var; expr.var out_var])
+        k_impl
+      <{ pred (nlet_eq [out_var] v k) }>.
   Proof. prove_field_compilation. Qed.
 
-  Lemma compile_inv :
-    forall (locals: Semantics.locals) (mem: Semantics.mem)
-           (locals_ok : Semantics.locals -> Prop)
-      tr retvars R Rin Rout functions T (pred: T -> list word -> Semantics.mem -> Prop)
-      (x : felem) x_ptr x_var out_ptr out_var (X : F M_pos) k k_impl,
-      spec_of_inv functions ->
-      bounded_by tight_bounds x ->
-      feval x = X ->
-      (FElem x_ptr x * Rin)%sep mem ->
-      (Placeholder out_ptr * Rout)%sep mem ->
-      map.get locals x_var = Some x_ptr ->
-      map.get locals out_var = Some out_ptr ->
-      let v := F.inv X in
-      (let head := v in
-       forall out m,
-         feval out = head ->
-         bounded_by loose_bounds out ->
-         sep (FElem out_ptr out) Rout m ->
-         (find k_impl
-          implementing (pred (k head))
-          and-returning retvars
-          and-locals-post locals_ok
-          with-locals locals and-memory m and-trace tr and-rest R
-          and-functions functions)) ->
-      (let head := v in
-       find (cmd.seq
-               (cmd.call [] inv [expr.var out_var; expr.var x_var])
-               k_impl)
-       implementing (pred (dlet head k))
-       and-returning retvars
-       and-locals-post locals_ok
-       with-locals locals and-memory mem and-trace tr and-rest R
-       and-functions functions).
-  Proof. prove_field_compilation. Qed.
+  Ltac cleanup_op_lemma lem := (* This makes [simple apply] work *)
+    let lm := fresh in
+    let op := match lem with _ _ ?op => op end in
+    let op_hd := term_head op in
+    let simp proj :=
+        (let hd := term_head proj in
+         let reduced := (eval cbv [op_hd hd] in proj) in
+         change proj with reduced in (type of lm)) in
+    pose lem as lm;
+    first [ simp (bin_model (BinOp := op));
+            simp (bin_xbounds (BinOp := op));
+            simp (bin_ybounds (BinOp := op));
+            simp (bin_outbounds (BinOp := op))
+          | simp (un_model (UnOp := op));
+            simp (un_xbounds (UnOp := op));
+            simp (un_outbounds (UnOp := op)) ];
+    let t := type of lm in
+    let t := (eval cbv beta in t) in
+    exact (lm: t).
 
-  Lemma compile_felem_copy :
-    forall (locals: Semantics.locals) (mem: Semantics.mem)
-           (locals_ok : Semantics.locals -> Prop)
-      tr retvars R R' functions T (pred: T -> list word -> Semantics.mem -> Prop)
-      (x : felem) x_ptr x_var out_ptr out_var
-      (X : F M_pos) k k_impl,
+  Notation make_bin_lemma op :=
+    ltac:(cleanup_op_lemma (@compile_binop _ op)) (only parsing).
+
+  Definition compile_mul := make_bin_lemma bin_mul.
+  Definition compile_add := make_bin_lemma bin_add.
+  Definition compile_sub := make_bin_lemma bin_sub.
+
+  Notation make_un_lemma op :=
+    ltac:(cleanup_op_lemma (@compile_unop _ op)) (only parsing).
+
+  Definition compile_square := make_un_lemma un_square.
+  Definition compile_scmula24 := make_un_lemma un_scmula24.
+  Definition compile_inv := make_un_lemma un_inv.
+
+  Lemma compile_felem_copy {tr mem locals functions} x :
+    let v := feval x in
+    forall {P} {pred: P v -> predicate} {k: nlet_eq_k P v} {k_impl}
+      R x_ptr x_var out_ptr out_var,
+
       spec_of_felem_copy functions ->
-      feval x = X ->
-      (FElem x_ptr x * Placeholder out_ptr * R')%sep mem ->
-      map.get locals x_var = Some x_ptr ->
+
       map.get locals out_var = Some out_ptr ->
-      let v := X in
-      (let head := v in
+
+      (FElem x_ptr x * Placeholder out_ptr * R)%sep mem ->
+      map.get locals x_var = Some x_ptr ->
+
+      (let v := v in
        forall m,
-         (FElem x_ptr x * FElem out_ptr x * R')%sep m ->
-         (find k_impl
-          implementing (pred (k head))
-          and-returning retvars
-          and-locals-post locals_ok
-          with-locals locals and-memory m and-trace tr and-rest R
-          and-functions functions)) ->
-      (let head := v in
-       find (cmd.seq
-               (cmd.call [] felem_copy [expr.var out_var; expr.var x_var])
-               k_impl)
-       implementing (pred (dlet head k))
-       and-returning retvars
-       and-locals-post locals_ok
-       with-locals locals and-memory mem and-trace tr and-rest R
-       and-functions functions).
+         (FElem x_ptr x * FElem out_ptr x * R)%sep m ->
+         (<{ Trace := tr;
+             Memory := m;
+             Locals := locals;
+             Functions := functions }>
+          k_impl
+          <{ pred (k v eq_refl) }>)) ->
+      <{ Trace := tr;
+         Memory := mem;
+         Locals := locals;
+         Functions := functions }>
+      cmd.seq
+        (cmd.call [] felem_copy [expr.var x_var; expr.var out_var])
+        k_impl
+      <{ pred (nlet_eq [out_var] v k) }>.
   Proof. prove_field_compilation. Qed.
 
-  Lemma compile_felem_small_literal :
-    forall (locals: Semantics.locals) (mem: Semantics.mem)
-           (locals_ok : Semantics.locals -> Prop)
-      tr retvars R R' functions T (pred: T -> list word -> Semantics.mem -> Prop)
-      (wx : word) (x : Z) out_ptr out_var k k_impl,
+  Lemma compile_felem_small_literal {tr mem locals functions} x:
+    let v := x mod M in
+    forall {P} {pred: P v -> predicate} {k: nlet_eq_k P v} {k_impl}
+      R (wx : word) (out : felem) out_ptr out_var,
+
       spec_of_felem_small_literal functions ->
-      (Placeholder out_ptr * R')%sep mem ->
+
       map.get locals out_var = Some out_ptr ->
+      (Placeholder out_ptr * R)%sep mem ->
+
       word.unsigned wx = x ->
-      let v := F.of_Z M_pos x in
-      (let head := v in
+
+      (let v := v in
        forall X m,
-         (FElem out_ptr X * R')%sep m ->
-         feval X = head ->
+         (FElem out_ptr X * R)%sep m ->
+         feval X = F.of_Z _ v ->
          bounded_by tight_bounds X ->
-         (find k_impl
-          implementing (pred (k head))
-          and-returning retvars
-          and-locals-post locals_ok
-          with-locals locals and-memory m and-trace tr and-rest R
-          and-functions functions)) ->
-      (let head := v in
-       find (cmd.seq
-               (cmd.call [] felem_small_literal
-                         [expr.var out_var; expr.literal x])
-               k_impl)
-       implementing (pred (dlet head k))
-       and-returning retvars
-       and-locals-post locals_ok
-       with-locals locals and-memory mem and-trace tr and-rest R
-       and-functions functions).
+         (<{ Trace := tr;
+             Memory := m;
+             Locals := locals;
+             Functions := functions }>
+          k_impl
+          <{ pred (k v eq_refl) }>)) ->
+      <{ Trace := tr;
+         Memory := mem;
+         Locals := locals;
+         Functions := functions }>
+      cmd.seq
+        (cmd.call [] felem_small_literal
+                  [expr.literal x; expr.var out_var])
+        k_impl
+      <{ pred (nlet_eq [out_var] v k) }>.
   Proof.
     prove_field_compilation.
     match goal with H : _ |- _ =>
                     rewrite word.of_Z_unsigned in H end.
     use_hyp_with_matching_cmd; eauto; [ ].
     subst_lets_in_goal.
-    match goal with H : F.to_Z _ = _ |- _ => rewrite <-H end.
-    rewrite F.of_Z_to_Z. eauto.
-  Qed.
-
-  (* noop indicating that the last argument should store output *)
-  Definition overwrite1 {A B} := @id (A -> B).
-  (* noop indicating that the 2nd-to-last argument should store output *)
-  Definition overwrite2 {A B C} := @id (A -> B -> C).
-
-  Lemma compile_compose_l :
-    forall (locals: Semantics.locals) (mem: Semantics.mem)
-           (locals_ok : Semantics.locals -> Prop)
-           tr retvars R Rout functions T (pred: T -> list word -> Semantics.mem -> Prop)
-           {A1 A2 : Type} (* second arg is N for F.pow, so allow that *)
-           (op1 : F M_pos -> A1 -> F M_pos)
-           (op2 : F M_pos -> A2 -> F M_pos)
-           x y z out_ptr out_var k k_impl,
-      (Placeholder out_ptr * Rout)%sep mem ->
-      map.get locals out_var = Some out_ptr ->
-      let v := ((op2 (op1 x y) z)) in
-      (let head := v in
-       (find k_impl
-        implementing
-             (pred (dlet (op1 x y)
-                         (fun xy => dlet ((overwrite2 op2) xy z) k)))
-        and-returning retvars
-        and-locals-post locals_ok
-        with-locals locals and-memory mem and-trace tr and-rest R
-        and-functions functions)) ->
-      (let head := v in
-       find k_impl
-       implementing (pred (dlet head k))
-       and-returning retvars
-       and-locals-post locals_ok
-       with-locals locals and-memory mem and-trace tr and-rest R
-       and-functions functions).
-  Proof.
-    cbv [Placeholder overwrite1 overwrite2] in *.
-    repeat straightline'. auto.
-  Qed.
-
-  Lemma compile_compose_r :
-    forall (locals: Semantics.locals) (mem: Semantics.mem)
-           (locals_ok : Semantics.locals -> Prop)
-      tr retvars R Rout functions T (pred: T -> list word -> Semantics.mem -> Prop)
-           {A1 : Type} (* second arg is N for F.pow, so allow that *)
-           (op1 : F M_pos -> A1 -> F M_pos)
-           (op2 : F M_pos -> F M_pos -> F M_pos)
-           x y z out_ptr out_var k k_impl,
-      (Placeholder out_ptr * Rout)%sep mem ->
-      map.get locals out_var = Some out_ptr ->
-      let v := (op2 z (op1 x y)) in
-      (let head := v in
-       (find k_impl
-        implementing
-             (pred (dlet (op1 x y)
-                         (fun xy => dlet ((overwrite1 op2) z xy) k)))
-        and-returning retvars
-        and-locals-post locals_ok
-        with-locals locals and-memory mem and-trace tr and-rest R
-        and-functions functions)) ->
-      (let head := v in
-       find k_impl
-       implementing (pred (dlet head k))
-       and-returning retvars
-       and-locals-post locals_ok
-       with-locals locals and-memory mem and-trace tr and-rest R
-       and-functions functions).
-  Proof.
-    cbv [Placeholder overwrite1 overwrite2] in *.
-    repeat straightline'. auto.
-  Qed.
-
-  Lemma compile_overwrite1 :
-    forall (locals: Semantics.locals) (mem: Semantics.mem)
-           (locals_ok : Semantics.locals -> Prop)
-      tr retvars R Rin functions T (pred: T -> list word -> Semantics.mem -> Prop)
-      (x : F M_pos) (op : F M_pos -> F M_pos -> F M_pos)
-      (y : felem) y_ptr y_var (Y : F M_pos) k k_impl,
-      (FElem y_ptr y * Rin)%sep mem ->
-      feval y = Y ->
-      map.get locals y_var = Some y_ptr ->
-      let v := (overwrite1 op) x Y in
-      let v' := op x Y in
-      (let __ := 0 in (* placeholder *)
-       forall m,
-         sep (FElem y_ptr y) Rin m ->
-         sep (Placeholder y_ptr) Rin m ->
-         (find k_impl
-          implementing (pred (dlet v' k))
-          and-returning retvars
-          and-locals-post locals_ok
-          with-locals locals and-memory m and-trace tr and-rest R
-          and-functions functions)) ->
-      (let head := v in
-       find k_impl
-       implementing (pred (dlet head k))
-       and-returning retvars
-       and-locals-post locals_ok
-       with-locals locals and-memory mem and-trace tr and-rest R
-       and-functions functions).
-  Proof.
-    repeat straightline'. auto.
-    match goal with H : _ |- _ => apply H end.
-    { ecancel_assumption. }
-    { seprewrite FElem_from_bytes.
-      sepsimpl; eexists; ecancel_assumption. }
-  Qed.
-
-  Lemma compile_overwrite2 :
-    forall (locals: Semantics.locals) (mem: Semantics.mem)
-           (locals_ok : Semantics.locals -> Prop)
-      tr retvars R Rin functions T (pred: T -> list word -> Semantics.mem -> Prop)
-      {A} (y : A)
-      (op : F M_pos -> A -> F M_pos)
-      (x : felem) x_ptr x_var (X : F M_pos) k k_impl,
-      feval x = X ->
-      (FElem x_ptr x * Rin)%sep mem ->
-      map.get locals x_var = Some x_ptr ->
-      let v := (overwrite2 op) X y in
-      let v' := op X y in
-      (let __ := 0 in (* placeholder *)
-       forall m,
-         sep (FElem x_ptr x) Rin m ->
-         sep (Placeholder x_ptr) Rin m ->
-         (find k_impl
-          implementing (pred (dlet v' k))
-          and-returning retvars
-          and-locals-post locals_ok
-          with-locals locals and-memory m and-trace tr and-rest R
-          and-functions functions)) ->
-      (let head := v in
-       find k_impl
-       implementing (pred (dlet head k))
-       and-returning retvars
-       and-locals-post locals_ok
-       with-locals locals and-memory mem and-trace tr and-rest R
-       and-functions functions).
-  Proof.
-    repeat straightline'. auto.
-    match goal with H : _ |- _ => apply H end.
-    { ecancel_assumption. }
-    { seprewrite FElem_from_bytes.
-      sepsimpl; eexists; ecancel_assumption. }
+    cbv [M]. rewrite <-F.of_Z_mod.
+    assumption.
   Qed.
 End Compile.
 
@@ -482,13 +215,6 @@ Ltac field_compile_step :=
   | |- feval _ = _ => try eassumption; try reflexivity
   | |- _ => idtac
   end.
-
-Ltac compile_compose_step :=
-  first [ simple eapply compile_compose_l
-        | simple eapply compile_compose_r
-        | simple eapply compile_overwrite1
-        | simple eapply compile_overwrite2 ];
-  [ solve [repeat compile_step] .. | intros ].
 
 (* Change an FElem into a Placeholder to indicate that it is overwritable *)
 Ltac free p :=
