src/Bedrock/Specs/Field.v
@@ -73,94 +73,111 @@ Class FieldRepresentation_ok
       forall X : felem, bounded_by tight_bounds X
                         -> bounded_by loose_bounds X;
   }.
-
-Notation unop_spec name op xbounds outbounds :=
-  (forall! (x : felem) (px pout : word),
-      (fun Rr mem =>
-         bounded_by xbounds x
-         /\ (exists Ra, (FElem px x * Ra)%sep mem)
-         /\ (Placeholder pout * Rr)%sep mem)
-        ===> name @ [pout; px] ===>
-        (fun _ =>
-           liftexists out,
-           (emp (feval out = op (feval x)
-                 /\ bounded_by outbounds out)
-            * FElem pout out)%sep))
-    (only parsing).
-
-Notation binop_spec name op xbounds ybounds outbounds :=
-  (forall! (x y : felem) (px py pout : word),
-      (fun Rr mem =>
-         bounded_by xbounds x
-         /\ bounded_by ybounds y
-         /\ (exists Ra, (FElem px x * Ra)%sep mem)
-         /\ (exists Ra, (FElem py y * Ra)%sep mem)
-         /\ (Placeholder pout * Rr)%sep mem)
-        ===> name @ [pout; px; py] ===>
-        (fun _ =>
-           liftexists out,
-           (emp ((feval out = op (feval x) (feval y))
-                 /\ bounded_by outbounds out)
-            * FElem pout out)%sep)) (only parsing).
-
 Section FunctionSpecs.
   Context {semantics : Semantics.parameters}
           {semantics_ok : Semantics.parameters_ok semantics}.
   Context {field_parameters : FieldParameters}
           {field_representaton : FieldRepresentation}.
 
-  Instance spec_of_mul : spec_of mul :=
-    binop_spec mul F.mul loose_bounds loose_bounds tight_bounds.
-  Instance spec_of_square : spec_of square :=
-    unop_spec square (fun x => F.mul x x) loose_bounds tight_bounds.
-  Instance spec_of_add : spec_of add :=
-    binop_spec add F.add tight_bounds tight_bounds loose_bounds.
-  Instance spec_of_sub : spec_of sub :=
-    binop_spec sub F.sub tight_bounds tight_bounds loose_bounds.
-  Instance spec_of_scmula24 : spec_of scmula24 :=
-    unop_spec scmula24 (F.mul a24) loose_bounds tight_bounds.
-  (* TODO: what are the bounds for inv? *)
-  Instance spec_of_inv : spec_of inv :=
-    unop_spec inv F.inv tight_bounds loose_bounds.
+  Class UnOp (name: string) :=
+    { un_model: F M_pos -> F M_pos;
+      un_xbounds: bounds;
+      un_outbounds: bounds }.
 
-  Definition spec_of_from_bytes : spec_of from_bytes :=
-    forall! (bs : list byte) (px pout : word),
-      (fun Rr mem =>
-         (exists Ra, (FElemBytes px bs * Ra)%sep mem)
-         /\ (Placeholder pout * Rr)%sep mem)
-        ===> from_bytes @ [pout; px] ===>
-        (fun _ =>
-           liftexists X,
-           (emp (feval X = feval_bytes bs /\ bounded_by tight_bounds X)
-            * FElem pout X)%sep).
+  Definition unop_spec {name} (op: UnOp name) :=
+    fnspec! name (px pout : word) / (x : felem) Rr,
+    { requires tr mem :=
+        bounded_by un_xbounds x
+        /\ (exists Ra, (FElem px x * Ra)%sep mem)
+        /\ (Placeholder pout * Rr)%sep mem;
+      ensures tr' mem' :=
+        tr = tr' /\
+        exists out,
+          feval out = un_model (feval x)
+          /\ bounded_by un_outbounds out
+          /\ (FElem pout out * Rr)%sep mem' }.
 
-  Definition spec_of_to_bytes : spec_of to_bytes :=
-    forall! (x : felem) (px pout : word) (old_out : list byte),
-      (fun Rr mem =>
-         bounded_by tight_bounds x
-         /\ (exists Ra, (FElem px x * Ra)%sep mem)
-         /\ (FElemBytes pout old_out * Rr)%sep mem)
-        ===> to_bytes @ [pout; px] ===>
-        (fun _ =>
-           liftexists bs,
-           (emp (feval_bytes bs = feval x) * FElemBytes pout bs)%sep).
+  Instance spec_of_UnOp {name} (op: UnOp name) : spec_of name :=
+    unop_spec op.
 
-  Definition spec_of_felem_copy : spec_of felem_copy :=
-    forall! (x : felem) (px pout : word),
-      (sep (FElem px x * Placeholder pout)%sep)
-        ===> felem_copy @ [pout; px] ===>
-        (fun _ => FElem px x * FElem pout x)%sep.
+  Class BinOp (name: string) :=
+    { bin_model: F M_pos -> F M_pos -> F M_pos;
+      bin_xbounds: bounds;
+      bin_ybounds: bounds;
+      bin_outbounds: bounds }.
 
-  Definition spec_of_felem_small_literal : spec_of felem_small_literal :=
-    forall! (x pout : word),
-      (sep (Placeholder pout))
-        ===> felem_small_literal @ [pout; x] ===>
-        (fun _ =>
-           liftexists X,
-           (emp (F.to_Z (feval X) = word.unsigned x
-                 /\ bounded_by tight_bounds X)
-            * FElem pout X)%sep).
+  Definition binop_spec  {name} (op: BinOp name) :=
+    fnspec! name (px py pout : word) / (x y: felem) Rr,
+    { requires tr mem :=
+        bounded_by bin_xbounds x
+        /\ bounded_by bin_ybounds y
+        /\ (exists Ra, (FElem px x * FElem py y * Ra)%sep mem)
+        /\ (Placeholder pout * Rr)%sep mem;
+      ensures tr' mem' :=
+        tr = tr' /\
+        exists out,
+          feval out = bin_model (feval x) (feval y)
+          /\ bounded_by bin_outbounds out
+          /\ (FElem pout out * Rr)%sep mem' }.
+
+  Instance spec_of_BinOp {name} (op: BinOp name) : spec_of name :=
+    binop_spec op.
+
+  Instance bin_mul : BinOp mul :=
+    {| bin_model := F.mul; bin_xbounds := loose_bounds; bin_ybounds := loose_bounds; bin_outbounds := tight_bounds |}.
+  Instance un_square : UnOp square :=
+    {| un_model := fun x => F.pow x 2; un_xbounds := loose_bounds; un_outbounds := tight_bounds |}.
+  Instance bin_add : BinOp add :=
+    {| bin_model := F.add; bin_xbounds := tight_bounds; bin_ybounds := tight_bounds; bin_outbounds := loose_bounds |}.
+  Instance bin_sub : BinOp sub :=
+    {| bin_model := F.sub; bin_xbounds := tight_bounds; bin_ybounds := tight_bounds; bin_outbounds := loose_bounds |}.
+  Instance un_scmula24 : UnOp scmula24 :=
+    {| un_model := F.mul a24; un_xbounds := loose_bounds; un_outbounds := tight_bounds |}.
+  Instance un_inv : UnOp inv := (* TODO: what are the bounds for inv? *)
+    {| un_model := F.inv; un_xbounds := tight_bounds; un_outbounds := loose_bounds |}.
+
+  Instance spec_of_from_bytes : spec_of from_bytes :=
+    fnspec! from_bytes (px pout : word) / (bs : list byte) Rr,
+    { requires tr mem :=
+        (exists Ra, (FElemBytes px bs * Ra)%sep mem)
+        /\ (Placeholder pout * Rr)%sep mem;
+      ensures tr' mem' :=
+        tr = tr' /\
+        exists X, feval X = feval_bytes bs
+             /\ bounded_by tight_bounds X
+             /\ (FElem pout X * Rr)%sep mem' }.
+
+  Instance spec_of_to_bytes : spec_of to_bytes :=
+    fnspec! to_bytes (px pout : word) / (x : felem) (old_out : list byte) Rr,
+    { requires tr mem :=
+        (exists Ra, (FElem px x * Ra)%sep mem)
+        /\ (FElemBytes pout old_out * Rr)%sep mem;
+      ensures tr' mem' :=
+        tr = tr' /\
+        exists bs, feval_bytes bs = feval x
+                   /\ (FElemBytes pout bs * Rr)%sep mem' }.
+
+  Instance spec_of_felem_copy : spec_of felem_copy :=
+    fnspec! felem_copy (px pout : word) / (x : felem) R,
+    { requires tr mem :=
+        (FElem px x * Placeholder pout * R)%sep mem;
+      ensures tr' mem' :=
+        tr = tr' /\
+        (FElem px x * FElem pout x * R)%sep mem' }.
+
+  Instance spec_of_felem_small_literal : spec_of felem_small_literal :=
+    fnspec! felem_small_literal (x pout : word) / R,
+    { requires tr mem :=
+        (Placeholder pout * R)%sep mem;
+      ensures tr' mem' :=
+        tr = tr' /\
+        exists X, feval X = F.of_Z _ (word.unsigned x)
+             /\ bounded_by tight_bounds X
+             /\ (FElem pout X * R)%sep mem' }.
 End FunctionSpecs.
+
+Existing Instances spec_of_UnOp spec_of_BinOp bin_mul un_square bin_add bin_sub
+         un_scmula24 un_inv spec_of_felem_copy spec_of_felem_small_literal.
 
 Section SpecProperties.
   Context {semantics : Semantics.parameters}
