src/Bedrock/Group/ScalarMult/LadderStep.v
@@ -11,9 +11,6 @@ Section __.
   Context {field_parameters : FieldParameters}
           {field_representaton : FieldRepresentation}
           {field_representation_ok : FieldRepresentation_ok}.
-  Existing Instances spec_of_mul spec_of_square spec_of_add
-           spec_of_sub spec_of_scmula24 spec_of_inv spec_of_felem_copy
-           spec_of_felem_small_literal.
   Hint Resolve relax_bounds : compiler.
 
   Section Gallina.
@@ -23,54 +20,28 @@ Section __.
                (X1: F M_pos) (P1 P2: point)  : (point * point) :=
       let '(X2, Z2) := P1 in
       let '(X3, Z3) := P2 in
-      let/d A := X2+Z2 in
-      let/d AA := A^2 in
-      let/d B := X2-Z2 in
-      let/d BB := B^2 in
-      let/d E := AA-BB in
-      let/d C := X3+Z3 in
-      let/d D := X3-Z3 in
-      let/d DA := D*A in
-      let/d CB := C*B in
-      let/d X5 := (DA+CB)^2 in
-      let/d Z5 := X1*(DA-CB)^2 in
-      let/d X4 := AA*BB in
-      let/dZ4 := E*(AA + a24*E) in
+      let/n A := X2+Z2 in
+      let/n AA := A^2 in
+      let/n B := X2-Z2 in
+      let/n BB := B^2 in
+      let/n E := AA-BB in
+      let/n C := X3+Z3 in
+      let/n D := X3-Z3 in
+      let/n DA := D*A in
+      let/n CB := C*B in
+      let/n X5 := (DA+CB)^2 in
+      let/n Z5 := X1*(DA-CB)^2 in
+      let/n X4 := AA*BB in
+      let/n Z4 := E*(AA + a24*E) in
       ((X4, Z4), (X5, Z5)).
   End Gallina.
 
-  (* single predicate for all ladderstep end-state information *)
-  (* N.B. it's important to leave the associativity of the predicate so that the
-     emp is separated from the rest. This way, sepsimpl can easily pull it
-     out. If sepsimpl is improved to handle very nested emps, this will not be
-     necessary. *)
-  Definition LadderStepResult
-             (X1 X2 Z2 X3 Z3 : felem)
-             (pX1 pX2 pZ2 pX3 pZ3 : Semantics.word)
-             (pA pAA pB pBB pE pC pD pDA pCB : Semantics.word)
-             (result : point * point)
-    : list word -> Semantics.mem -> Prop :=
-    fun _ =>
-      (liftexists X4 Z4 X5 Z5 (* output values *)
-                  A' AA' B' BB' E' C' D' DA' CB' (* new intermediates *)
-       : felem,
-         (emp (result = ((feval X4, feval Z4), (feval X5, feval Z5))
-               /\ bounded_by tight_bounds X4
-               /\ bounded_by tight_bounds Z4
-               /\ bounded_by tight_bounds X5
-               /\ bounded_by tight_bounds Z5)
-          * (FElem pX1 X1 * FElem pX2 X4 * FElem pZ2 Z4
-             * FElem pX3 X5 * FElem pZ3 Z5
-             * FElem pA A' * FElem pAA AA'
-             * FElem pB B' * FElem pBB BB'
-             * FElem pE E' * FElem pC C' * FElem pD D'
-             * FElem pDA DA' * FElem pCB CB'))%sep).
-
   Instance spec_of_ladderstep : spec_of "ladderstep" :=
-    forall! (X1 X2 Z2 X3 Z3 : felem)
+    fnspec! "ladderstep"
           (pX1 pX2 pZ2 pX3 pZ3
-               pA pAA pB pBB pE pC pD pDA pCB : Semantics.word),
-      (fun R m =>
+               pA pAA pB pBB pE pC pD pDA pCB : Semantics.word)
+          / (X1 X2 Z2 X3 Z3 : felem) R,
+    { requires tr mem :=
         bounded_by tight_bounds X1
         /\ bounded_by tight_bounds X2
         /\ bounded_by tight_bounds Z2
@@ -83,47 +54,94 @@ Section __.
             * Placeholder pB * Placeholder pBB
             * Placeholder pE * Placeholder pC
             * Placeholder pD * Placeholder pDA
-            * Placeholder pCB * R)%sep m)
-        ===>
-        "ladderstep" @ [pX1; pX2; pZ2; pX3; pZ3; pA; pAA; pB; pBB; pE; pC; pD; pDA; pCB]
-        ===>
-        (LadderStepResult
-           X1 X2 Z2 X3 Z3 pX1 pX2 pZ2 pX3 pZ3
-           pA pAA pB pBB pE pC pD pDA pCB
-           (ladderstep_gallina
-              (feval X1) (feval X2, feval Z2)
-              (feval X3, feval Z3))).
+            * Placeholder pCB * R)%sep mem;
+      ensures tr' mem' :=
+        tr = tr'
+        /\ exists X4 Z4 X5 Z5 (* output values *)
+               A' AA' B' BB' E' C' D' DA' CB' (* new intermediates *)
+               : felem,
+          (ladderstep_gallina
+             (feval X1) (feval X2, feval Z2)
+             (feval X3, feval Z3)
+           = ((feval X4, feval Z4), (feval X5, feval Z5)))
+          /\ bounded_by tight_bounds X4
+          /\ bounded_by tight_bounds Z4
+          /\ bounded_by tight_bounds X5
+          /\ bounded_by tight_bounds Z5
+          /\ (FElem pX1 X1 * FElem pX2 X4 * FElem pZ2 Z4
+              * FElem pX3 X5 * FElem pZ3 Z5
+              * FElem pA A' * FElem pAA AA'
+              * FElem pB B' * FElem pBB BB'
+              * FElem pE E' * FElem pC C' * FElem pD D'
+              * FElem pDA DA' * FElem pCB CB' * R)%sep mem'}.
 
-    Lemma compile_ladderstep :
-      forall (locals: Semantics.locals) (mem: Semantics.mem)
-        (locals_ok : Semantics.locals -> Prop)
-        tr retvars R R' functions T (pred: T -> _ -> _ -> Prop)
-        x1 x2 z2 x3 z3
-        X1 X1_ptr X1_var X2 X2_ptr X2_var Z2 Z2_ptr Z2_var
-        X3 X3_ptr X3_var Z3 Z3_ptr Z3_var
-        A_ptr A_var AA_ptr AA_var B_ptr B_var BB_ptr BB_var
-        E_ptr E_var C_ptr C_var D_ptr D_var
-        DA_ptr DA_var CB_ptr CB_var
-        k k_impl,
-        spec_of_ladderstep functions ->
-        feval X1 = x1 ->
-        feval X2 = x2 ->
-        feval Z2 = z2 ->
-        feval X3 = x3 ->
-        feval Z3 = z3 ->
-        bounded_by tight_bounds X1 ->
-        bounded_by tight_bounds X2 ->
-        bounded_by tight_bounds Z2 ->
-        bounded_by tight_bounds X3 ->
-        bounded_by tight_bounds Z3 ->
-        (FElem X1_ptr X1
-         * FElem X2_ptr X2 * FElem Z2_ptr Z2
-         * FElem X3_ptr X3 * FElem Z3_ptr Z3
-         * Placeholder A_ptr * Placeholder AA_ptr
-         * Placeholder B_ptr * Placeholder BB_ptr
-         * Placeholder E_ptr * Placeholder C_ptr
-         * Placeholder D_ptr * Placeholder DA_ptr
-         * Placeholder CB_ptr * R')%sep mem ->
+  (*
+    let v := un_model (eval x) mod M in
+    forall {P} {pred: P v -> predicate} {k: nlet_eq_k P v} {k_impl}
+      Rin Rout (out : bignum) x_ptr x_var out_ptr out_var,
+
+      (_: spec_of name) functions ->
+      bounded_by un_xbounds x ->
+
+      map.get locals out_var = Some out_ptr ->
+      (Placeholder out_ptr out * Rout)%sep mem ->
+
+      (Bignum x_ptr x * Rin)%sep mem ->
+      map.get locals x_var = Some x_ptr ->
+
+      (let v := v in
+       forall out m (Heq: eval out mod M = v),
+         bounded_by un_outbounds out ->
+         sep (Bignum out_ptr out) Rout m ->
+         (<{ Trace := tr;
+             Memory := m;
+             Locals := locals;
+             Functions := functions }>
+          k_impl
+          (* <{ (rew [fun v => P v -> predicate)] Heq in pred) (k (eval out mod M) Heq) }>)) -> *)
+          <{ pred (k v eq_refl) }>)) ->
+      <{ Trace := tr;
+         Memory := mem;
+         Locals := locals;
+         Functions := functions }>
+      cmd.seq
+        (cmd.call [] name [expr.var x_var; expr.var out_var])
+        k_impl
+      <{ pred (nlet_eq [out_var] v k) }>.
+   *)
+  Print nlet_eq.
+  Lemma compile_ladderstep {tr mem locals functions}
+        (x1 x2 z2 x3 z3 : F M_pos) :
+    let v := ladderstep_gallina x1 (x2, z2) (x3, z3) in
+    forall {P} {pred: P v -> predicate} {k: nlet_eq_k P v} {k_impl}
+           Rout
+           X1 X1_ptr X1_var X2 X2_ptr X2_var Z2 Z2_ptr Z2_var
+           X3 X3_ptr X3_var Z3 Z3_ptr Z3_var
+           A_ptr A_var AA_ptr AA_var B_ptr B_var BB_ptr BB_var
+           E_ptr E_var C_ptr C_var D_ptr D_var
+           DA_ptr DA_var CB_ptr CB_var,
+
+      spec_of_ladderstep functions ->
+
+      feval X1 = x1 ->
+      feval X2 = x2 ->
+      feval Z2 = z2 ->
+      feval X3 = x3 ->
+      feval Z3 = z3 ->
+      bounded_by tight_bounds X1 ->
+      bounded_by tight_bounds X2 ->
+      bounded_by tight_bounds Z2 ->
+      bounded_by tight_bounds X3 ->
+      bounded_by tight_bounds Z3 ->
+      (FElem X1_ptr X1
+       * FElem X2_ptr X2 * FElem Z2_ptr Z2
+       * FElem X3_ptr X3 * FElem Z3_ptr Z3
+       * Placeholder A_ptr * Placeholder AA_ptr
+       * Placeholder B_ptr * Placeholder BB_ptr
+       * Placeholder E_ptr * Placeholder C_ptr
+       * Placeholder D_ptr * Placeholder DA_ptr
+       * Placeholder CB_ptr * Rout)%sep mem ->
+
         map.get locals X1_var = Some X1_ptr ->
         map.get locals X2_var = Some X2_ptr ->
         map.get locals Z2_var = Some Z2_ptr ->
@@ -138,46 +156,59 @@ Section __.
         map.get locals D_var = Some D_ptr ->
         map.get locals DA_var = Some DA_ptr ->
         map.get locals CB_var = Some CB_ptr ->
-        let v := ladderstep_gallina x1 (x2, z2) (x3, z3) in
-        (let head := v in
-         forall m,
-           (LadderStepResult
-             X1 X2 Z2 X3 Z3 X1_ptr X2_ptr Z2_ptr X3_ptr
-             Z3_ptr A_ptr AA_ptr B_ptr BB_ptr E_ptr C_ptr D_ptr DA_ptr
-             CB_ptr head [] * R')%sep m ->
-           (find k_impl
-            implementing (pred (k head))
-            and-returning retvars
-            and-locals-post locals_ok
-            with-locals locals
-            and-memory m and-trace tr and-rest R
-            and-functions functions)) ->
-        (let head := v in
-         find (cmd.seq
-                 (cmd.call [] "ladderstep"
-                           [ expr.var X1_var; expr.var X2_var;
-                               expr.var Z2_var; expr.var X3_var;
-                                 expr.var Z3_var; expr.var A_var;
-                                   expr.var AA_var; expr.var B_var;
-                                     expr.var BB_var; expr.var E_var;
-                                       expr.var C_var; expr.var D_var;
-                                         expr.var DA_var; expr.var CB_var ])
 
-                 k_impl)
-         implementing (pred (dlet head k))
-         and-returning retvars
-         and-locals-post locals_ok
-         with-locals locals
-         and-memory mem and-trace tr and-rest R
-         and-functions functions).
+        (let v := v in
+         forall (X4 Z4 X5 Z5 (* output values *)
+                    A' AA' B' BB' E' C' D' DA' CB' (* new intermediates *)
+                 : felem) m
+                (Heq : ladderstep_gallina
+                         (feval X1) (feval X2, feval Z2)
+                         (feval X3, feval Z3)
+                       = ((feval X4, feval Z4), (feval X5, feval Z5))),
+          bounded_by tight_bounds X4 ->
+          bounded_by tight_bounds Z4 ->
+          bounded_by tight_bounds X5 ->
+          bounded_by tight_bounds Z5 ->
+          (FElem X1_ptr X1 * FElem X2_ptr X4 * FElem Z2_ptr Z4
+           * FElem X3_ptr X5 * FElem Z3_ptr Z5
+           * FElem A_ptr A' * FElem AA_ptr AA'
+           * FElem B_ptr B' * FElem BB_ptr BB'
+           * FElem E_ptr E' * FElem C_ptr C' * FElem D_ptr D'
+           * FElem DA_ptr DA' * FElem CB_ptr CB' * Rout)%sep m ->
+           (<{ Trace := tr;
+               Memory := m;
+               Locals := locals;
+               Functions := functions }>
+            k_impl
+            <{ pred (k v eq_refl) }>)) ->
+
+        <{ Trace := tr;
+           Memory := mem;
+           Locals := locals;
+           Functions := functions }>
+        cmd.seq
+          (cmd.call [] "ladderstep"
+                    [ expr.var X1_var; expr.var X2_var;
+                        expr.var Z2_var; expr.var X3_var;
+                          expr.var Z3_var; expr.var A_var;
+                            expr.var AA_var; expr.var B_var;
+                              expr.var BB_var; expr.var E_var;
+                                expr.var C_var; expr.var D_var;
+                                  expr.var DA_var; expr.var CB_var ])
+          k_impl
+        <{ pred (nlet_eq
+                   [X1_var; X2_var; Z2_var; X3_var; Z3_var]
+                   v k) }>.
     Proof.
       repeat straightline'.
-      handle_call; [ solve [eauto] .. | sepsimpl ].
-      repeat straightline'. subst. eauto.
+      handle_call;
+        lazymatch goal with
+        | |- sep _ _ _ => ecancel_assumption
+        | _ => solve [eauto]
+        end.
     Qed.
 
   Ltac ladderstep_compile_custom :=
-    repeat compile_compose_step;
     field_compile_step; [ repeat compile_step .. | ];
     (* if the output we selected was one of the inputs, need to write the
        Placeholder back into a FElem for the arguments precondition *)
@@ -194,15 +225,28 @@ Section __.
   Derive ladderstep_body SuchThat
          (let args := ["X1"; "X2"; "Z2"; "X3"; "Z3";
                          "A"; "AA"; "B"; "BB"; "E"; "C";
-                           "D"; "DA"; "CB"] in
-          let ladderstep := ("ladderstep", (args, [], ladderstep_body)) in
-          program_logic_goal_for
-            ladderstep
-            (ltac:(let x := program_logic_goal_for_function
-                              ladderstep [mul;add;sub;square;scmula24] in
-                   exact x)))
-    As ladderstep_body_correct.
+                         "D"; "DA"; "CB"] in
+          ltac:(
+            let proc := constr:(("ladderstep",
+                                 (args, [], ladderstep_body))
+                                : Syntax.func) in
+            let goal := Rupicola.Lib.Tactics.program_logic_goal_for_function
+                          proc [mul;add;sub;square;scmula24] in
+            exact (__rupicola_program_marker ladderstep_gallina -> goal)))
+         As ladderstep_correct.
   Proof.
+    compile_setup.
+
+    repeat (simple apply compile_nlet_as_nlet_eq;
+            repeat compile_step).
+
+    Check compile_square.
+    Print compile_step.
+    compile_cleanup.
+    field_compile_step.
+    1-8:repeat
+    compile_step.
+    repeat compile_step.
     cbv [program_logic_goal_for spec_of_ladderstep].
     setup.
     repeat safe_compile_step.
